Mind be broken, proofs are hard

project.v
@@ -11,16 +11,16 @@ Inductive sorted : @Tree nat -> Prop :=
   | leaf_sorted : sorted null
   | node_empty (t : nat) : sorted (node t null null)
   | node_left (t l : nat) (ll lr : Tree) :
-      (l <=? t) = true ->
+      (l <? t) = true ->
       sorted (node l ll lr) ->
       sorted (node t (node l ll lr) null)
   | node_right (t r : nat) (rl rr : Tree) :
-      (t <=? r) = true ->
+      (t <? r) = true ->
       sorted (node r rl rr) ->
       sorted (node t null (node r rl rr))
   | node_full (t l r : nat) (ll lr rl rr : Tree) :
-      (l <=? t) = true ->
-      (t <=? r) = true ->
+      (l <? t) = true ->
+      (t <? r) = true ->
       sorted (node l ll lr) ->
       sorted (node r rl rr) ->
       sorted (node t (node l ll lr) (node r rl rr)).
@@ -40,3 +40,87 @@ Fixpoint elem_of (x : nat) (t : @Tree nat) : bool := match t with
     if x <? t then elem_of x l else elem_of x r
   | null => false
 end.
+
+Example SortedDoesntContain4 : elem_of 4 Sorted = false.
+Proof. reflexivity. Qed.
+
+Example SortedDoesntContain27 : elem_of 27 Sorted = false.
+Proof. reflexivity. Qed.
+
+Example SortedContains17 : elem_of 17 Sorted = true.
+Proof. reflexivity. Qed.
+
+Example SortedContains10 : elem_of 10 Sorted = true.
+Proof. reflexivity. Qed.
+
+Fixpoint insert (x : nat) (t : Tree) : Tree := match t with
+  | node t l r => if x =? t then node t l r else
+    if x <? t then node t (insert x l) r else node t l (insert x r)
+  | null => node x null null
+end.
+
+Example InsertIntoEmpty : insert 5 null = node 5 null null.
+Proof. reflexivity. Qed.
+
+Example InsertIntoExisting : insert 7 (insert 5 null) = node 5 null (node 7 null null).
+Proof. reflexivity. Qed.
+
+Lemma insert_always_produce_node : forall t x,
+  exists t' l r, insert x t = node t' l r.
+Proof.
+  induction t.
+  - intros x. unfold insert. destruct (x =? t1). {
+      exists t1. exists t2. exists t3. reflexivity.
+    }
+    destruct (x <? t1). {
+      destruct (IHt1 x). exists t1. destruct H. destruct H.
+      exists (node x0 x1 x2). exists t3. rewrite <- H. reflexivity.
+    }
+    exists t1. exists t2. destruct (IHt2 x). destruct H. destruct H.
+    exists (node x0 x1 x2). rewrite <- H. reflexivity.
+  - intros x. exists x. exists null. exists null. reflexivity.
+Qed.
+
+Lemma insert_diff_root_stays :
+  forall (x x': nat) (t1 t2 : Tree),
+  x' <> x ->
+  exists (t1' t2' : Tree), insert x' (node x t1 t2) = node x t1' t2'.
+Proof.
+  intros.
+Admitted.
+
+Lemma subst_node : forall (x' : nat) (t : Tree),
+  insert x' t = node x' null null \/
+  (exists (x : nat) (t1 t2 t1': Tree), t = node x t1 t2 -> x' <? x = true -> insert x' t = node x t1' t2) \/
+  (exists (x : nat) (t1 t2 : Tree), t = node x t1 t2 -> x = x' -> insert x' t = t) \/
+  (exists (x : nat) (t1 t2 t2' : Tree), t = node x t1 t2 -> x <? x' = true -> insert x' t = node x t1 t2').
+Proof.
+Admitted.
+
+Lemma insert_sorted : forall t x,
+  sorted t -> sorted (insert x t).
+Proof.
+  induction t.
+  - intros. cbn. destruct (x =? t1) eqn:Heq. {
+    apply H.
+  }
+  destruct t1.
+    + destruct t2. {
+        inversion H. inversion H2. inversion H4.
+      }
+      destruct t3. 2: {
+        constructor.
+        - destruct x.
+          + discriminate Heq.
+          + reflexivity.
+        - constructor.
+      }
+      inversion H. apply (IHt2 x) in H5. subst.
+
+        apply (IHt2 x) in H5.
+      assert (Hsome_node: exists (n : nat) (t1' t2': Tree),
+              insert x (node t t3_1 t3_2) = node n t1' t2'). {
+        apply insert_always_produce_node.
+      }
+      destruct Hsome_node as [x' [t1' [t2']]].
+      rewrite H6 in *. constructor. subst.
